formalization/BasicTypingProp.v
@@ -11,19 +11,75 @@ Import BasicTyping.
 Import Trace.
 Import OperationalSemantics.
 
-Lemma basic_typing_weaken_value: forall Γ Γ' (v: value) T,
-    Γ ⊆ Γ' -> Γ ⊢t v ⋮v T -> Γ' ⊢t v ⋮v T.
-Admitted.
-
 Lemma basic_typing_weaken_tm: forall Γ Γ' (v: tm) T,
-    Γ ⊆ Γ' -> Γ ⊢t v ⋮t T -> Γ' ⊢t v ⋮t T.
-Admitted.
+    Γ ⊆ Γ' -> Γ ⊢t v ⋮t T -> Γ' ⊢t v ⋮t T
+with basic_typing_weaken_value: forall Γ Γ' (v: value) T,
+    Γ ⊆ Γ' -> Γ ⊢t v ⋮v T -> Γ' ⊢t v ⋮v T.
+Proof.
+  all : intros * Hs; destruct 1; econstructor; eauto using lookup_weaken.
+  all: instantiate_atom_listctx;
+    auto_eapply;
+    try lazymatch goal with
+      | |- _ ⊆ _ => apply insert_mono; eauto
+      | _ => eauto
+      end.
+Qed.
 
-Lemma basic_typing_subst_value: forall Γ z u U (v: value) T, Γ ⊢t u ⋮v U -> <[z := U]> Γ ⊢t v ⋮v T -> Γ ⊢t {z := u}v v ⋮v T.
-Admitted.
+Lemma basic_typing_weaken_insert_tm: forall Γ (v: tm) T x U,
+    x # Γ -> Γ ⊢t v ⋮t T -> <[x := U]>Γ ⊢t v ⋮t T.
+Proof.
+  intros. eapply basic_typing_weaken_tm. 2: eauto.
+  apply insert_subseteq. apply not_elem_of_dom. my_set_solver.
+Qed.
+
+Lemma basic_typing_weaken_insert_value: forall Γ (v: value) T x U,
+    x # Γ -> Γ ⊢t v ⋮v T -> <[x := U]> Γ ⊢t v ⋮v T.
+Proof.
+  intros. eapply basic_typing_weaken_value. 2: eauto.
+  apply insert_subseteq. apply not_elem_of_dom. my_set_solver.
+Qed.
 
 Lemma basic_typing_subst_tm: forall Γ z u U (v: tm) T, Γ ⊢t u ⋮v U -> <[z := U]> Γ ⊢t v ⋮t T -> Γ ⊢t {z := u}t v ⋮t T.
-Admitted.
+Proof.
+  intros * Hu Ht; remember (<[z:=U]> Γ); revert dependent Γ.
+  revert c v T Ht.
+  apply (tm_has_type_mutual_rec
+           (fun c v T _ => ∀ Γ : context, Γ ⊢t u ⋮v U → c = <[z:=U]> Γ → Γ ⊢t {z := u }v v ⋮v T)
+           (fun c v T _ => ∀ Γ : context, Γ ⊢t u ⋮v U → c = <[z:=U]> Γ → Γ ⊢t {z := u }t v ⋮t T)); intros; subst; simpl in *; eauto; try econstructor; eauto.
+  case_decide; subst.
+  (* For some reason normal rewrite does not work. *)
+  setoid_rewrite lookup_insert in e. simplify_eq. eauto.
+  econstructor. setoid_rewrite lookup_insert_ne in e; eauto.
+
+  all:
+  instantiate_atom_listctx;
+  rewrite <- subst_open_var_tm by
+    (eauto using basic_typing_regular_value; my_set_solver);
+  auto_eapply; [
+      eapply basic_typing_weaken_insert_value; eauto; my_set_solver
+    | apply insert_commute; my_set_solver ].
+Qed.
+
+Lemma basic_typing_subst_value: forall Γ z u U (v: value) T, Γ ⊢t u ⋮v U -> <[z := U]> Γ ⊢t v ⋮v T -> Γ ⊢t {z := u}v v ⋮v T.
+Proof.
+  intros * Hu Ht; remember (<[z:=U]> Γ); revert dependent Γ.
+  revert c v T Ht.
+  apply (value_has_type_mutual_rec
+           (fun c v T _ => ∀ Γ : context, Γ ⊢t u ⋮v U → c = <[z:=U]> Γ → Γ ⊢t {z := u }v v ⋮v T)
+           (fun c v T _ => ∀ Γ : context, Γ ⊢t u ⋮v U → c = <[z:=U]> Γ → Γ ⊢t {z := u }t v ⋮t T)); intros; subst; simpl in *; eauto; try econstructor; eauto.
+  case_decide; subst.
+  (* For some reason normal rewrite does not work. *)
+  setoid_rewrite lookup_insert in e. simplify_eq. eauto.
+  econstructor. setoid_rewrite lookup_insert_ne in e; eauto.
+
+  all:
+  instantiate_atom_listctx;
+  rewrite <- subst_open_var_tm by
+    (eauto using basic_typing_regular_value; my_set_solver);
+  auto_eapply; [
+      eapply basic_typing_weaken_insert_value; eauto; my_set_solver
+    | apply insert_commute; my_set_solver ].
+Qed.
 
 Lemma eval_op_type_safe: forall α op (v1 v: constant) (T1 T: base_ty),
     α ⊧{ op ~ v1 }⇓{ v } ->
